matching-logic/src/Theories/Definedness_ProofSystem.v
@@ -15,7 +15,7 @@ From Coq.Classes Require Import Morphisms_Prop.
 From Coq.Unicode Require Import Utf8.
 From Coq.micromega Require Import Lia.
 
-From MatchingLogic Require Import Syntax NamedAxioms DerivedOperators_Syntax ProofSystem ProofMode IndexManipulation.
+From MatchingLogic Require Import Syntax NamedAxioms DerivedOperators_Syntax ProofSystem ProofMode IndexManipulation Substitution.
 From MatchingLogic.Theories Require Import Definedness_Syntax.
 From MatchingLogic.Utils Require Import stdpp_ext.
 
@@ -1873,7 +1873,6 @@ apply Framing_right.
 exact H.
 Defined.
 
-
 Lemma floor_monotonic {Σ : Signature} {syntax : Syntax} Γ ϕ₁ ϕ₂ :
 theory ⊆ Γ ->
 well_formed ϕ₁ ->
@@ -3115,4 +3114,145 @@ apply phi_impl_total_phi_meta.
 toMyGoal.
 { wf_auto2. }
 mgIntro. mgLeft. mgExactn 0.
+Defined.
+
+Lemma bott_not_total {Σ : Signature} {syntax : Syntax}:
+  forall Γ, theory ⊆ Γ ->
+  Γ ⊢ ! ⌊ ⊥ ⌋.
+Proof.
+  intros Γ SubTheory.
+  toMyGoal. wf_auto2.
+  mgIntro. mgApply 0.
+  mgApplyMeta (@phi_impl_defined_phi _ _ _ (! ⊥) SubTheory ltac:(wf_auto2)).
+  mgIntro. mgExactn 1.
+Defined.
+
+Lemma defined_not_iff_not_total {Σ : Signature} {syntax : Syntax}:
+  ∀ (Γ : Theory) (ϕ : Pattern),
+  theory ⊆ Γ → well_formed ϕ → Γ ⊢ ⌈ ! ϕ ⌉ <---> ! ⌊ ϕ ⌋.
+Proof.
+  intros Γ φ HΓ Wf. toMyGoal. wf_auto2.
+  mgSplitAnd.
+  * mgIntro. mgApplyMeta (@def_not_phi_impl_not_total_phi _ _ Γ φ HΓ Wf). mgExactn 0.
+  * unfold patt_total.
+    pose proof (@not_not_iff _ Γ ⌈ ! φ ⌉ ltac:(wf_auto2)) as H.
+    mgRewrite <- H at 1. mgIntro. mgExactn 0.
+Defined.
+
+Lemma patt_or_total {Σ : Signature} {syntax : Syntax}:
+  forall Γ φ ψ,
+  theory ⊆ Γ ->
+  well_formed φ -> well_formed ψ ->
+  Γ ⊢  ⌊ φ ⌋ or ⌊ ψ ⌋ ---> ⌊ φ or ψ ⌋.
+Proof.
+  intros Γ φ ψ HΓ Wf1 Wf2. toMyGoal. wf_auto2.
+  mgIntro. mgDestructOr 0.
+  * pose proof (@disj_left_intro _ Γ φ ψ Wf1 Wf2) as H.
+    apply floor_monotonic in H. 2-4: try wf_auto2.
+    mgApplyMeta H. mgExactn 0.
+  * pose proof (@disj_right_intro _ Γ φ ψ Wf1 Wf2) as H.
+    apply floor_monotonic in H. 2-4: try wf_auto2.
+    mgApplyMeta H. mgExactn 0.
+Defined.
+
+Lemma patt_defined_and {Σ : Signature} {syntax : Syntax}:
+  forall Γ φ ψ,
+  theory ⊆ Γ ->
+  well_formed φ -> well_formed ψ ->
+  Γ ⊢ ⌈ φ and ψ ⌉ ---> ⌈ φ ⌉ and ⌈ ψ ⌉.
+Proof.
+  intros Γ φ ψ HΓ Wf1 Wf2. toMyGoal. wf_auto2.
+  unfold patt_and.
+  mgRewrite (@defined_not_iff_not_total _ _ Γ (! φ or ! ψ) HΓ ltac:(wf_auto2)) at 1.
+  do 2 mgIntro. mgApply 0. mgClear 0.
+  mgApplyMeta (@patt_or_total _ _ _ (! φ) (! ψ) HΓ ltac:(wf_auto2) ltac:(wf_auto2)).
+  mgDestructOr 0.
+  * mgLeft. unfold patt_total.
+    mgRewrite <- (@not_not_iff _ Γ φ Wf1) at 1. mgExactn 0.
+  * mgRight. unfold patt_total.
+    mgRewrite <- (@not_not_iff _ Γ ψ Wf2) at 1. mgExactn 0.
+Defined.
+
+Lemma patt_total_and {Σ : Signature} {syntax : Syntax}:
+  forall Γ φ ψ,
+  theory ⊆ Γ ->
+  well_formed φ -> well_formed ψ ->
+  Γ ⊢ ⌊ φ and ψ ⌋ <---> ⌊ φ ⌋ and ⌊ ψ ⌋.
+Proof.
+  intros Γ φ ψ HΓ Wf1 Wf2. toMyGoal. wf_auto2.
+  mgSplitAnd.
+  * unfold patt_and.
+    mgRewrite <- (@def_propagate_not _ _ Γ (! φ or ! ψ) HΓ ltac:(wf_auto2)) at 1.
+    mgIntro. mgIntro. mgApply 0.
+    mgClear 0.
+    mgRewrite (@ceil_compat_in_or _ _ Γ (! φ) (! ψ) HΓ ltac:(wf_auto2) ltac:(wf_auto2)) at 1.
+    mgDestructOr 0.
+    - mgLeft. mgRevert. unfold patt_total.
+      mgRewrite <- (@not_not_iff _ Γ ⌈ ! φ ⌉ ltac:(wf_auto2)) at 1.
+      mgIntro. mgExactn 0.
+    - mgRight. mgRevert. unfold patt_total.
+      mgRewrite <- (@not_not_iff _ Γ ⌈ ! ψ ⌉ ltac:(wf_auto2)) at 1.
+      mgIntro. mgExactn 0.
+  * mgIntro. mgDestructAnd 0.
+    unfold patt_and.
+    mgRewrite <- (@def_propagate_not _ _ Γ (! φ or ! ψ) HΓ ltac:(wf_auto2)) at 1.
+    mgRewrite (@ceil_compat_in_or _ _ Γ (! φ) (! ψ) HΓ ltac:(wf_auto2) ltac:(wf_auto2)) at 1.
+    mgIntro. mgDestructOr 2.
+    - mgRevert. mgExactn 0.
+    - mgRevert. mgExactn 1.
+Defined.
+
+Lemma defined_variables_equal {Σ : Signature} {syntax : Syntax} :
+  forall x y Γ,
+  theory ⊆ Γ ->
+  Γ ⊢ ⌈ patt_free_evar y and patt_free_evar x ⌉ ---> patt_free_evar y =ml patt_free_evar x.
+Proof.
+  intros x y Γ HΓ.
+  toMyGoal. wf_auto2.
+  unfold patt_equal, patt_iff.
+  pose proof (@patt_total_and _ _ _
+                                (patt_free_evar y ---> patt_free_evar x)
+                                (patt_free_evar x ---> patt_free_evar y) HΓ ltac:(wf_auto2) ltac:(wf_auto2)) as H.
+  apply pf_iff_proj2 in H. 2-3: wf_auto2.
+  mgIntro.
+  mgApplyMeta H. clear H.
+  mgIntro. mgDestructOr 1.
+  * mgApply 1. mgClear 1. mgIntro.
+    pose proof (H := @ProofMode.nimpl_eq_and _ Γ (patt_free_evar y) (patt_free_evar x)
+                  ltac:(wf_auto2) ltac:(wf_auto2)).
+    epose proof (H0 := @prf_equiv_congruence _ Γ 
+    _ _ {| pcEvar := x; pcPattern := ⌈ patt_free_evar x ⌉  |} ltac:(wf_auto2) H).
+    cbn in H0. case_match. 2: congruence.
+    apply pf_iff_proj1 in H0. 2-3: wf_auto2.
+    mgApplyMeta H0 in 1.
+    (* TODO: it is increadibly inconvienient to define concrete contexts *)
+    pose proof (H1 := @Singleton_ctx _ Γ 
+           (@ctx_app_r _ (patt_sym (Definedness_Syntax.inj definedness)) box 
+                ltac:(wf_auto2))
+           (@ctx_app_r _ (patt_sym (Definedness_Syntax.inj definedness)) box 
+                ltac:(wf_auto2)) (patt_free_evar x) y ltac:(wf_auto2)).
+    mgApplyMeta H1. simpl. mgSplitAnd. mgExactn 0. mgExactn 1.
+  * mgApply 1. mgClear 1. mgIntro.
+    pose proof (H := @ProofMode.nimpl_eq_and _ Γ (patt_free_evar x) (patt_free_evar y)
+                  ltac:(wf_auto2) ltac:(wf_auto2)).
+    epose proof (H0 := @prf_equiv_congruence _ Γ 
+    _ _ {| pcEvar := x; pcPattern := ⌈ patt_free_evar x ⌉  |} ltac:(wf_auto2) H).
+    cbn in H0. case_match. 2: congruence.
+    apply pf_iff_proj1 in H0. 2-3: wf_auto2.
+    mgApplyMeta H0 in 1.
+    (* TODO: mgRewriteBy does not work for free evars :( *)
+    pose proof (H1 := @patt_and_comm _ Γ (patt_free_evar y) (patt_free_evar x) ltac:(wf_auto2) ltac:(wf_auto2)).
+    epose proof (H2 := @prf_equiv_congruence _ Γ 
+    _ _ {| pcEvar := x; pcPattern := ⌈ patt_free_evar x ⌉  |} ltac:(wf_auto2) H1).
+    cbn in H2. case_match. 2: congruence.
+    apply pf_iff_proj1 in H2. 2-3: wf_auto2.
+    mgAssert (⌈ patt_free_evar x and patt_free_evar y ⌉). wf_auto2.
+    mgClear 1. mgApplyMeta H2. mgExactn 0.
+    (* TODO: it is increadibly inconvienient to define concrete contexts *)
+    pose proof (@Singleton_ctx _ Γ 
+           (@ctx_app_r _ (patt_sym (Definedness_Syntax.inj definedness)) box 
+                ltac:(wf_auto2))
+           (@ctx_app_r _ (patt_sym (Definedness_Syntax.inj definedness)) box 
+                ltac:(wf_auto2)) (patt_free_evar y) x ltac:(wf_auto2)) as H3.
+    mgApplyMeta H3. simpl. mgSplitAnd. mgExactn 2. mgExactn 1.
 Defined.
