matching-logic/src/Theories/Unification.v
@@ -1,0 +1,566 @@
+From Coq Require Import ssreflect ssrfun ssrbool.
+Set Implicit Arguments.
+Unset Strict Implicit.
+Unset Printing Implicit Defensive.
+
+From Ltac2 Require Import Ltac2.
+
+Require Import Equations.Prop.Equations.
+
+From Coq Require Import String Ensembles Setoid.
+Require Import Coq.Program.Equality.
+Require Import Coq.Logic.Classical_Prop.
+From Coq.Logic Require Import FunctionalExtensionality Eqdep_dec.
+From Coq.Classes Require Import Morphisms_Prop.
+From Coq.Unicode Require Import Utf8.
+From Coq.micromega Require Import Lia.
+
+From MatchingLogic Require Import Syntax NamedAxioms DerivedOperators_Syntax ProofSystem ProofMode IndexManipulation Substitution.
+From MatchingLogic.Theories Require Import Definedness_Syntax Definedness_ProofSystem.
+From MatchingLogic.Utils Require Import stdpp_ext.
+
+Require Import MatchingLogic.wftactics.
+
+From stdpp Require Import base fin_sets sets propset proof_irrel option list.
+
+Import extralibrary.
+
+Import MatchingLogic.Syntax.Notations.
+Import MatchingLogic.DerivedOperators_Syntax.Notations.
+Import MatchingLogic.Syntax.BoundVarSugar.
+Import MatchingLogic.ProofSystem.Notations.
+
+Set Default Proof Mode "Classic".
+
+Close Scope equations_scope. (* Because of [!] *)
+
+Import Notations.
+Open Scope ml_scope.
+
+Section ProofSystemTheorems.
+  Context
+    {Σ : Signature}
+    {syntax : Syntax}.
+
+  Lemma Prop₃_left: forall Γ φ φ',
+      theory ⊆ Γ -> mu_free φ ->
+      well_formed φ -> well_formed φ' ->
+      Γ ⊢ (φ and (φ' =ml φ)) ---> (φ and φ').
+  Proof.
+    intros Γ φ φ' SubTheory Mufree Wf1 Wf2.
+    toMyGoal. wf_auto2.
+    mgIntro. mgDestructAnd 0.
+    mgRewriteBy 1 at 1. auto. wf_auto.
+    mgSplitAnd; mgExactn 0.
+  Defined.
+
+  Lemma membership_imp_equal :
+    forall Γ φ φ',
+      theory ⊆ Γ -> mu_free φ' ->
+      well_formed φ -> well_formed φ' ->
+      Γ ⊢ (ex , (φ =ml b0)) ->
+      Γ ⊢ (ex , (φ' =ml b0)) ->
+      Γ ⊢ (φ ∈ml φ') ---> (φ =ml φ').
+  Proof.
+    intros Γ φ φ' HΓ Mufree Wf1 Wf2 Funφ Funφ'.
+    unfold patt_in, patt_equal.
+    toMyGoal. wf_auto2.
+
+    (* TODO: proposal: functional_reasoning tactic, which replaces a pattern with a 
+                       free variable *)
+    epose proof (@forall_functional_subst _ _ (⌈ b0 and φ' ⌉ ---> ⌊ b0 <---> φ' ⌋) φ 
+                    Γ HΓ ltac:(wf_auto2) ltac:(wf_auto2) _ ltac:(wf_auto2)) as H.
+    Unshelve. 2: { cbn. case_match; auto. apply andb_true_iff in Wf2 as [_ Wf2].
+                   apply andb_true_iff in Wf2 as [_ Wf2].
+                   (* NOTE: using eapply breaks the proof *)
+                   apply well_formed_closed_ex_aux_ind with (ind_evar2 := 1)in Wf2.
+                   rewrite Wf2. auto. lia. } (* TODO: this should be auto... *)
+    simpl in H.
+    repeat rewrite bevar_subst_not_occur in H. wf_auto2. (* TODO: cast_proof? *)
+    mgApplyMeta H. clear H.
+    mgSplitAnd. 2: fromMyGoal; wf_auto2.
+    epose proof (@forall_functional_subst _ _ (all, (⌈ b0 and b1 ⌉ ---> ⌊ b0 <---> b1 ⌋)) φ'
+                    Γ HΓ ltac:(wf_auto2) ltac:(wf_auto2) _ ltac:(wf_auto2)) as H.
+    Unshelve. 2: { cbn. do 2 case_match; auto; lia. }
+    mgApplyMeta H. clear H.
+
+    mgSplitAnd. 2: fromMyGoal; wf_auto2.
+    remember (fresh_evar patt_bott) as x.
+    remember (fresh_evar (patt_free_evar x)) as y.
+    assert (x <> y) as XY.
+    { intro. apply x_eq_fresh_impl_x_notin_free_evars in Heqy.
+      subst. set_solver. } (* TODO: this should be auto... *)
+    fromMyGoal. wf_auto2.
+
+
+   (* TODO: mgIntro for supporting 'all' *)
+
+
+    pose proof (@universal_generalization _ Γ (all , (⌈ b0 and patt_free_evar x ⌉ ---> ⌊ b0 <---> patt_free_evar x ⌋)) x ltac:(wf_auto2)) as H1.
+    simpl in H1. case_match; auto. apply H1. clear H1.
+    pose proof (@universal_generalization _ Γ (⌈ (patt_free_evar y) and (patt_free_evar x) ⌉ ---> ⌊ (patt_free_evar y) <---> (patt_free_evar x) ⌋) y ltac:(wf_auto2)) as H1.
+    simpl in H1. clear H Heqs. do 2 case_match; auto; try congruence.
+    2-3: exfalso; apply n; reflexivity. (* TODO: congruence does not work... *)
+    apply H1. clear H1.
+    now apply defined_variables_equal.
+  Defined.
+
+  Lemma functional_pattern_defined :
+    forall Γ φ, theory ⊆ Γ -> well_formed φ ->
+       Γ ⊢ (ex , (φ =ml b0)) ---> ⌈ φ ⌉.
+  Proof.
+    intros Γ φ HΓ Wf.
+    toMyGoal. wf_auto2.
+    mgIntro.
+    mgApplyMeta (@forall_functional_subst _ _ ⌈ b0 ⌉ φ _ HΓ ltac:(wf_auto2)
+                 ltac:(wf_auto2) ltac:(wf_auto2) ltac:(wf_auto2)).
+    mgSplitAnd.
+    * mgClear 0. fromMyGoal. wf_auto2.
+      remember (fresh_evar patt_bott) as x.
+      pose proof (@universal_generalization _ Γ ⌈patt_free_evar x⌉ x ltac:(wf_auto2)) 
+        as H1.
+      cbn in H1. case_match. 2: congruence. apply H1.
+      now apply defined_evar.
+    * mgExactn 0.
+  Defined.
+
+  Lemma equal_imp_membership :
+    forall Γ φ φ',
+      theory ⊆ Γ -> mu_free φ' ->
+      well_formed φ -> well_formed φ' ->
+      Γ ⊢ ⌈ φ' ⌉ ->
+      Γ ⊢ (φ =ml φ') ---> (φ ∈ml φ').
+  Proof.
+    intros Γ φ φ' HΓ MF WF1 WF2 Def.
+    toMyGoal. wf_auto2.
+    mgIntro.
+    mgRewriteBy 0 at 1; cbn; wf_auto2.
+      mgClear 0. unfold patt_in.
+      assert (Γ ⊢ ( φ' and φ' <---> φ')) as H1.
+      {
+        toMyGoal. wf_auto2.
+        mgSplitAnd; mgIntro.
+        - mgDestructAnd 0. mgExactn 0.
+        - mgSplitAnd; mgExactn 0.
+      }
+      now mgRewrite H1 at 1.
+  Defined.
+
+  Lemma membership_equal_equal :
+    forall Γ φ φ',
+      theory ⊆ Γ -> mu_free φ' ->
+      well_formed φ -> well_formed φ' ->
+      Γ ⊢ (ex , (φ =ml b0)) ->
+      Γ ⊢ (ex , (φ' =ml b0)) ->
+      Γ ⊢ (φ ∈ml φ') =ml (φ =ml φ').
+  Proof.
+    intros Γ φ φ' HΓ Mufree Wf1 Wf2 Func1 Func2.
+    unfold patt_equal at 1.
+
+    toMyGoal. wf_auto2.
+    mgIntro.
+    mgApplyMeta (@bott_not_defined _ _ Γ).
+    fromMyGoal. wf_auto2.
+    
+    apply ceil_monotonic; auto. wf_auto2.
+
+    toMyGoal. wf_auto2.
+    mgApplyMeta (@not_not_intro _ Γ ((φ ∈ml φ' <---> φ =ml φ' ))
+                    ltac:(wf_auto2)).
+    mgSplitAnd; mgIntro.
+    * mgApplyMeta (membership_imp_equal HΓ Mufree Wf1 Wf2 Func1 Func2). mgExactn 0.
+    * mgApplyMeta (equal_imp_membership HΓ Mufree Wf1 Wf2 _). mgExactn 0.
+      Unshelve.
+      toMyGoal. wf_auto2.
+      now mgApplyMeta (functional_pattern_defined HΓ Wf2).
+  Defined.
+
+  Lemma Prop₃_right : forall Γ φ φ',
+      theory ⊆ Γ ->
+      well_formed φ -> well_formed φ' -> mu_free φ' ->
+      Γ ⊢ (ex , (φ =ml b0)) ->
+      Γ ⊢ (ex , (φ' =ml b0)) ->
+      Γ ⊢ (φ and φ') ---> (φ and (φ =ml φ')).
+  Proof.
+    intros Γ φ φ' HΓ Wf1 Wf2 MF Func1 Func2.
+    toMyGoal. wf_auto2.
+    mgIntro.
+    mgAssert (⌈ φ and φ' ⌉). wf_auto2.
+    (* Why can we only mgApplyMeta here, and not after mgRevert? *)
+    mgApplyMeta (@phi_impl_defined_phi Σ syntax Γ (φ and φ') HΓ ltac:(wf_auto2)).
+    mgExactn 0.
+    replace (⌈ φ and φ' ⌉) with (φ ∈ml φ') by auto.
+    mgDestructAnd 0. mgSplitAnd.
+    * mgExactn 0.
+    * mgApplyMeta (membership_imp_equal HΓ MF Wf1 Wf2 Func1 Func2).
+      mgExactn 2.
+  Defined.
+
+  Corollary delete : forall φ φ' Γ,
+    well_formed φ -> well_formed φ'
+  ->
+    Γ ⊢ φ and φ' =ml φ' ---> φ.
+  Proof.
+    intros φ φ' Γ WF1 WF2.
+    toMyGoal. wf_auto2.
+    mgIntro. mgDestructAnd 0. mgExactn 0.
+  Defined.
+
+  Lemma free_evar_subst_id :
+    forall φ x, φ.[[evar: x ↦ patt_free_evar x]] = φ.
+  Proof.
+    induction φ; intros x'; simpl; auto.
+    * case_match; subst; auto.
+    * rewrite IHφ1. now rewrite IHφ2.
+    * rewrite IHφ1. now rewrite IHφ2.
+    * now rewrite IHφ.
+    * now rewrite IHφ.
+  Qed.
+
+  Theorem elimination : forall φ φ' x Γ, x ∉ free_evars φ ->
+    theory ⊆ Γ -> mu_free φ ->
+    well_formed_closed_ex_aux φ 1 ->
+    well_formed_closed_mu_aux φ 0 ->
+    well_formed φ' ->
+    Γ ⊢ φ.[evar: 0 ↦ patt_free_evar x] and φ' =ml patt_free_evar x ---> 
+        φ.[evar: 0 ↦ φ'] and φ' =ml patt_free_evar x.
+  Proof.
+    intros φ φ' x Γ NotIn HΓ MF WFp1 WFp2 WF2.
+    assert (well_formed (φ.[evar:0↦φ'])) as WFF.
+    { wf_auto2. apply bevar_subst_positive; auto.
+        now apply mu_free_wfp. }
+    assert (well_formed (φ.[evar:0↦patt_free_evar x])) as WFFF. {
+      wf_auto2. apply bevar_subst_positive; auto.
+        now apply mu_free_wfp. }
+    toMyGoal. wf_auto2.
+    mgIntro. mgDestructAnd 0. mgSplitAnd. 2: mgExactn 1.
+    epose proof (@equality_elimination_basic _ _ Γ φ' (patt_free_evar x)
+            {|pcEvar := x; pcPattern := φ.[evar: 0 ↦ patt_free_evar x]|} 
+            HΓ WF2 ltac:(wf_auto2) ltac:(wf_auto2) ltac:(wf_auto2)).
+    cbn in H.
+    pose proof (@bound_to_free_variable_subst _ φ x 1 0 φ' ltac:(lia) ltac:(wf_auto2) WFp1 NotIn) as H0.
+    unfold evar_open in H0. rewrite <- H0 in H. (* TODO: cast_proof? *)
+    rewrite free_evar_subst_id in H.
+    assert (Γ ⊢ φ.[evar:0↦φ'] <---> φ.[evar:0↦patt_free_evar x] --->
+                φ.[evar:0↦patt_free_evar x] ---> φ.[evar:0↦φ']) as Hiff. {
+      toMyGoal; wf_auto2.
+      mgIntro. unfold patt_iff. mgDestructAnd 0. mgExactn 1.
+    }
+    epose proof (@syllogism_intro _ Γ _ _ _ _ _ _ H Hiff).
+    (* TODO: mgApplyMeta buggy?
+             Tries to match the longest conclusion, not the shortest *)
+    apply reorder_meta in H1.
+    mgRevert. mgApplyMeta H1. mgExactn 0.
+    Unshelve. all: wf_auto2.
+    cbn. rewrite mu_free_bevar_subst; wf_auto2.
+  Defined.
+
+  Theorem elimination_reverse : forall φ φ' x Γ, x ∉ free_evars φ ->
+    theory ⊆ Γ -> mu_free φ ->
+    well_formed_closed_ex_aux φ 1 ->
+    well_formed_closed_mu_aux φ 0 ->
+    well_formed φ' ->
+    Γ ⊢ φ.[evar: 0 ↦ φ'] and φ' =ml patt_free_evar x --->
+        φ.[evar: 0 ↦ patt_free_evar x] and φ' =ml patt_free_evar x.
+  Proof.
+    intros φ φ' x Γ NotIn HΓ MF WFp1 WFp2 WF2.
+    assert (well_formed (φ.[evar:0↦φ'])) as WFF.
+    { wf_auto2. apply bevar_subst_positive; auto.
+        now apply mu_free_wfp. }
+    assert (well_formed (φ.[evar:0↦patt_free_evar x])) as WFFF. {
+      wf_auto2. apply bevar_subst_positive; auto.
+        now apply mu_free_wfp. }
+    toMyGoal. wf_auto2.
+    mgIntro. mgDestructAnd 0. mgSplitAnd. 2: mgAssumption.
+    epose proof (@equality_elimination_basic _ _ Γ φ' (patt_free_evar x)
+            {|pcEvar := x; pcPattern := φ.[evar: 0 ↦ patt_free_evar x]|} 
+            HΓ WF2 ltac:(wf_auto2) ltac:(wf_auto2) ltac:(wf_auto2)).
+    cbn in H.
+    pose proof (@bound_to_free_variable_subst _ φ x 1 0 φ' ltac:(lia) ltac:(wf_auto2) WFp1 NotIn) as H0.
+    unfold evar_open in H0. rewrite <- H0 in H. (* TODO: cast_proof? *)
+    rewrite free_evar_subst_id in H.
+    assert (Γ ⊢ φ.[evar:0↦φ'] <---> φ.[evar:0↦patt_free_evar x] --->
+                φ.[evar:0↦φ'] ---> φ.[evar:0↦patt_free_evar x]) as Hiff. {
+      toMyGoal; wf_auto2.
+      mgIntro. unfold patt_iff. mgDestructAnd 0. mgExactn 0.
+    }
+    epose proof (@syllogism_intro _ Γ _ _ _ _ _ _ H Hiff).
+    (* TODO: mgApplyMeta buggy?
+             Tries to match the longest conclusion, not the shortest *)
+    apply reorder_meta in H1.
+    mgRevert. mgApplyMeta H1. mgExactn 0.
+    Unshelve. all: wf_auto2.
+    cbn. rewrite mu_free_bevar_subst; wf_auto2.
+  Defined.
+
+
+
+
+  (**
+     Should be a consequence of the injectivity axiom:
+
+      f(x₁,...,xₙ) = f(x₁',...,xₙ') → x₁ = x₁' ∧ ... ∧ xₙ = xₙ'
+
+     The question is, why can we assume this axiom?
+  *)
+  Definition application_chain (φ : Pattern) (φs : list Pattern) : Pattern :=
+    fold_left (fun Acc φ => patt_app Acc φ) φs φ.
+
+  Theorem application_equal : forall φs ψ φ's Γ,
+    length φs = length φ's ->
+    well_formed ψ -> (* Forall well_formed φs -> Forall well_formed φ's *)
+    (forall i, i < length φs -> well_formed (nth i φs ⊥)) ->
+    (forall i, i < length φ's -> well_formed (nth i φ's ⊥))
+  ->
+    Γ ⊢ application_chain ψ φs =ml application_chain ψ φ's --->
+         fold_right (fun '(x, y) Acc => Acc and x =ml y) Top (zip φs φ's).
+  Proof.
+    induction φs;
+    intros ψ φ's Γ Len WF WFs1 WFs2.
+    * apply eq_sym, length_zero_iff_nil in Len. subst. cbn.
+      toMyGoal. wf_auto2. mgIntro. mgClear 0. (* TODO: mgExact for meta theorems *)
+      fromMyGoal. wf_auto2.
+      apply (top_holds Γ).
+    * destruct φ's. simpl in Len. congruence.
+      simpl in Len. inversion Len. clear Len.
+      cbn.
+      admit.
+  Abort.
+
+End ProofSystemTheorems.
+
+Section UnificationProcedure.
+  Context {Σ : Signature} {ΣS : Syntax}.
+
+  (* Fixpoint apps_r (C : Application_context) : bool :=
+  match C with
+   | box => true
+   | ctx_app_l cc p => apps_r cc
+   | ctx_app_r p cc => false
+  end. *)
+
+  (** Based on https://www.cs.bu.edu/fac/snyder/publications/UnifChapter.pdf *)
+  Definition Unification_problem : Set := list (Pattern * Pattern) * 
+                                          list (evar * Pattern).
+
+  Fixpoint get_apps (p : Pattern) : option (symbols * list Pattern) :=
+  match p with
+  | patt_app p1 p2 =>
+    match get_apps p1 with
+    | Some (s, ps) => Some (s, ps ++ [p2])
+    | None => None
+    end
+  | patt_sym s => Some (s, [])
+  | _ => None
+  end.
+
+  Definition u_remove := remove (prod_eqdec Pattern_eqdec Pattern_eqdec).
+
+  Definition subst_ziplist (x : evar) (p : Pattern) 
+    : list (Pattern * Pattern) -> list (Pattern * Pattern) :=
+    map (fun '(p1, p2) => ( p1.[[evar: x ↦ p]] , p2.[[evar: x ↦ p]] )).
+  Definition subst_list (x : evar) (p : Pattern) 
+    : list (evar * Pattern) -> list (evar * Pattern) :=
+    map (fun '(y, p2) => ( y , p2.[[evar: x ↦ p]] )).
+
+  Reserved Notation "u ===> u'" (at level 80).
+  Inductive unify_step : Unification_problem -> option Unification_problem -> Set :=
+  (* trivial/delete *)
+  | u_trivial t U S U' :
+    (U ++ (t, t)::U', S) ===> Some (U ++ U', S)
+  (* decomposition *)
+  | u_decompose U U' S t1 t2 f ps ps' :
+    get_apps t1 = Some (f, ps) -> get_apps t2 = Some (f, ps') ->
+    length ps = length ps'
+   ->
+    (U ++ (t1, t2)::U', S) ===> Some (zip ps ps' ++ U ++ U', S)
+  (* symbol_clash *)
+  | u_clash U U' S t1 t2 f g ps ps' :
+    get_apps t1 = Some (f, ps) -> get_apps t2 = Some (g, ps') ->
+    f <> g
+   ->
+    (U ++ (t1, t2)::U', S) ===> None
+  (* orient *)
+  | u_orient U U' S t x:
+    (U ++ (t, patt_free_evar x)::U', S) ===> Some (U ++ (patt_free_evar x, t)::U', S)
+  (* occurs check *)
+  | u_check U U' S x t:
+    x ∈ free_evars t ->
+    patt_free_evar x <> t
+   ->
+    (U ++ (t, patt_free_evar x)::U', S) ===> None
+  (* elimination *)
+  | u_elim U U' S x t:
+    x ∉ free_evars t
+   ->
+    (U ++ (patt_free_evar x, t)::U', S) ===> Some (subst_ziplist x t (U ++ U'), 
+                                                   (x, t) :: subst_list x t S)
+  where "u ===> u'" := (unify_step u u').
+
+  Definition unification_to_pattern (u : Unification_problem) : Pattern :=
+    match u with
+    | (Us, Ss) => 
+        fold_right patt_and Top (map (fun '(p1, p2) => p1 =ml p2) Us)
+        and
+        fold_right patt_and Top (map (fun '(x, p2) => patt_free_evar x =ml p2) Ss)
+    end.
+
+  Definition wf_unification (u : Unification_problem) :=
+    (forall t1 t2, In (t1, t2) (fst u) -> well_formed t1 /\ well_formed t2) /\
+    (forall x t, In (x, t) (snd u) -> well_formed t).
+
+  Theorem foldr_equiv :
+    forall l p l' p0, well_formed p -> well_formed (foldr patt_and p0 l) -> well_formed (foldr patt_and p0 l') ->
+    forall Γ, Γ ⊢ foldr patt_and p0 (l ++ p::l') <---> foldr patt_and p0 (p::l ++ l').
+  Proof.
+    intros l. induction l; intros p l' p0 WFp WFl WFl' Γ.
+    * simpl. apply pf_iff_equiv_refl. wf_auto2.
+    * simpl.
+  Abort.
+
+  Theorem wf_unify_step :
+    forall u u' : Unification_problem,
+    u ===> Some u' ->
+    wf_unification u ->
+    wf_unification u'.
+  Proof.
+    intros u u' D. dependent induction D; intros WF; destruct WF as [WF1 WF2].
+    * split.
+      - intros t1 t2 HIn. simpl in HIn. apply in_app_or in HIn.
+        apply WF1. destruct HIn.
+        + now apply in_app_l.
+        + apply in_app_r. now constructor 2.
+      - intros x t0 HIn. simpl in HIn.
+        now apply (WF2 x).
+    * 
+  Abort.
+
+  Theorem wf_unify_pattern :
+    forall u, wf_unification u -> well_formed (unification_to_pattern u).
+  Proof.
+  Abort.
+
+  Theorem unification_soundness :
+    forall u u' : Unification_problem,
+    u ===> Some u' ->
+    wf_unification u ->
+    forall Γ, theory ⊆ Γ -> Γ ⊢ unification_to_pattern u ---> unification_to_pattern u'.
+  Proof.
+    intros u u' D WF.
+    assert (wf_unification u') as H.
+    { (* eapply wf_unify_step; eassumption. *) admit. }
+    dependent induction D; intros Γ HΓ.
+    * subst.
+      (* TODO: why does toMyGoal simplify??? *)
+      Opaque unification_to_pattern.
+      toMyGoal.
+      { (* apply well_formed_imp; apply wf_unify_pattern; auto. *) admit. }
+      Transparent unification_to_pattern.
+      cbn.
+      rewrite map_app. simpl map.
+      (* epose proof (@foldr_equiv (map (λ '(p1, p2), p1 =ml p2) U) (t =ml t) (map (λ '(p1, p2), p1 =ml p2) U') Top _ _ _ Γ).
+
+      mgIntro.
+      mgDestructAnd 0. mgSplitAnd. 2: mgAssumption. mgClear 1.
+      (* TODO: why can't be app folded back?
+               something is seriously wrong here *)
+      Search patt_and patt_imp ML_proof_system. *)
+      (* mgRewrite H0 at 1. *)
+     
+  Abort.
+
+
+
+
+
+
+
+
+
+
+
+
+
+
+
+
+
+
+
+
+
+
+
+
+(* (*   Axiom f : symbols.
+  Compute (get_apps (patt_sym f $ ⊥ $ ⊤ $ ⊥)). *)
+  Fixpoint unify_step1 (u : Unification_problem) : option Unification_problem :=
+  match u with
+  | []           => Some []
+  | (t1, t2)::xs =>
+    match unify_step1 xs with
+    | None => None
+    | Some xs' =>
+      match decide (t1 = t2) with
+      | left _ => Some xs' (* delete *)
+      | right _ =>
+        match get_apps t1, get_apps t2 with
+        | Some (s, ps), Some (s', ps') =>
+          match decide (s = s') with
+          | left _ => Some (xs' ++ zip ps ps') (* decomposition *)
+          | right _ => None (* symbol clash *)
+          end
+        | _, _ => Some xs'
+        end
+      end
+    end
+  end. *)
+
+  Definition is_free_evar (p : Pattern) : bool :=
+  match p with
+  | patt_free_evar _ => true
+  | _ => false
+  end.
+
+  Definition swap_if {A : Type} (P : A -> bool) (p : A * A): A * A :=
+  match p with
+  | (p1, p2) =>
+    match P p1, P p2 with
+    | true, _ => (p1, p2)
+    | _, true => (p2, p1)
+    | _, _    => (p1, p2)
+    end
+  end.
+
+  (* (* orient *)
+  Definition unify_step2 (u : Unification_problem) : Unification_problem :=
+     map (swap_if is_free_evar) u.
+
+  (* occurs_check *)
+  Fixpoint unify_step3 (u : Unification_problem) : option Unification_problem :=
+  match u with
+  | [] => Some []
+  | (p1, p2)::xs =>
+    match unify_step3 xs with
+    | Some xs' =>
+      match p1 with
+      | patt_free_evar x =>
+        match decide (x ∈ free_evars p2) with
+        | left _ => None
+        | right _ => Some ((p1, p2)::xs')
+        end
+      | _ => Some ((p1, p2)::xs')
+      end
+    | None => None
+    end
+  end.
+
+  (* 1x elimination *)
+  Fixpoint unify_step3 (u : Unification_problem) : Unification_problem :=
+  match u with
+  | [] => []
+  | (patt_free_evar x, p2)::xs => 
+  | (p1, p2)::xs => unify_step3 xs
+  end. *)
+
+End UnificationProcedure.
